ACL2Lean.lean
@@ -16,6 +16,7 @@ import ACL2Lean.ProofLog
 import ACL2Lean.ClauseId
 import ACL2Lean.ProofTree
 import ACL2Lean.ClauseTree
+import ACL2Lean.Imported.Lifting
 import ACL2Lean.Imported.SimpleWorld
 import ACL2Lean.Imported.NativeMirrors
 import ACL2Lean.Lexorder
